wip, with sheera

share/pulse/examples/PulseTree.fst
@@ -57,14 +57,14 @@ let rec is_tree #t (ct:tree_t t) (ft:T.tree t)
 //Whereas, intro is to prove the existence of the functional version from the concrete version.
 ```pulse
 ghost
-fn elim_is_tree_nil (#t:Type0) (x:tree_t t)
-requires is_tree x 'l ** pure ('l == T.Leaf) //elim is like from the LHS, we are getting the RHS
+fn elim_is_tree_leaf (#t:Type0) (x:tree_t t)
+requires is_tree x T.Leaf //elim is like from the LHS, we are getting the RHS
                                          //requires have the precondition that 'l is empty
                                          // And 'l comes from is_list x 'l
 ensures pure (x == None)                 // Just look at the RHS of l == [], that is the postcondition
 {
    //show_proof_state;
-   rewrite each 'l as T.Leaf #t; //each instance of such 'l is Nil; We are setting the context for empty lists
+  //  rewrite each 'l as T.Leaf #t; //each instance of such 'l is Nil; We are setting the context for empty lists
    //show_proof_state;
    unfold (is_tree x T.Leaf) // unfold exposes the definition of the function inside it. 
                          // is_list x [], RHS side is pure (x == None)
@@ -74,41 +74,33 @@ ensures pure (x == None)                 // Just look at the RHS of l == [], tha
 
 ```pulse
 ghost
-fn intro_is_tree_nil (#t:Type0) (x:tree_t t) // opposite to elim. elim is breakig, intro is assembling.
+fn intro_is_tree_leaf (#t:Type0) (x:tree_t t) // opposite to elim. elim is breakig, intro is assembling.
 requires pure (x == None) // From RHS
 ensures is_tree x T.Leaf // To LHS
 {
-    fold (is_tree x T.Leaf); //just take the LHS and fold it to create the LHS.
-}
-```
-```pulse
-ghost
-fn elim_is_tree_cons (#t:Type0) (ct:tree_t t) (ft:T.tree t) (data:t) (ltree:T.tree t) (rtree:T.tree t)
-requires is_tree ct ft ** pure (ft == T.Node data ltree rtree)
-ensures (
-  exists* (p:node_ptr t) (lct:tree_t t) (rct:tree_t t).
-    pure (ct == Some p) **
-    pts_to p { data = data; left = lct;right = rct } **
-    is_tree lct ltree **
-    is_tree rct rtree
-)
-{
-  rewrite each ft as (T.Node data ltree rtree);
-  rewrite_by
-    (is_tree ct (T.Node data ltree rtree))
-    (exists* (p:node_ptr t) (lct:tree_t t) (rct:tree_t t).
-      pure (ct == Some p) **
-      pts_to p { data = data; left = lct; right = rct } **
-      is_tree lct ltree **
-      is_tree rct rtree)
-    vprop_equiv_norm
-    ()
+  fold (is_tree x T.Leaf); //just take the LHS and fold it to create the LHS.
 }
 ```
 
 ```pulse
 ghost
-fn intro_is_tree_cons (#t:Type0) (ct:tree_t t) (v:node_ptr t) (#node:node t) (#ltree:T.tree t) (#rtree:T.tree t)
+fn elim_is_tree_node (#t:Type0) (ct:tree_t t) (data:t) (ltree:T.tree t) (rtree:T.tree t)
+requires is_tree ct (T.Node data ltree rtree)
+ensures (
+  exists* (p:node_ptr t) (lct:tree_t t) (rct:tree_t t).
+    pure (ct == Some p) **
+    pts_to p { data; left = lct;right = rct } **
+    is_tree lct ltree **
+    is_tree rct rtree
+)
+{
+  unfold is_tree
+}
+```
+
+```pulse
+ghost
+fn intro_is_tree_node (#t:Type0) (ct:tree_t t) (v:node_ptr t) (#node:node t) (#ltree:T.tree t) (#rtree:T.tree t)
 requires
   pts_to v node **
   is_tree node.left ltree **
@@ -117,18 +109,10 @@ requires
 ensures
   is_tree ct (T.Node node.data ltree rtree)
 {
-    rewrite (pts_to v node) as (pts_to v { data=node.data; left = node.left; right = node.right});
-    rewrite_by //fold is_tree ct (T.Node node.data ltree rtree) ---> This works now. Rebuild and see.
-        (exists* (p:node_ptr t) (lct:tree_t t) (rct:tree_t t).
-          pure (ct == Some p) **
-          pts_to p { data = node.data; left = lct; right = rct } **
-          is_tree lct ltree **
-          is_tree rct rtree)
-          (is_tree ct (T.Node node.data ltree rtree))
-           vprop_equiv_norm
-          ()
+  fold (is_tree ct (T.Node node.data ltree rtree))
 }
 ```
+
 //boilerplate$
 //is_tree_cases$
 let is_tree_cases #t (x:tree_t t) (ft: T.tree t)
@@ -150,20 +134,14 @@ requires is_tree x ft
 ensures  is_tree_cases x ft
 {
   match ft {
-    T.Leaf -> { 
-      elim_is_tree_nil x;
+    T.Leaf -> {
+      unfold (is_tree x T.Leaf);
       fold (is_tree_cases None ft);
-      rewrite each (None #(ref (node t))) as x;
     }
-    T.Node data ltree rtree -> { 
-      elim_is_tree_cons x ft data ltree rtree;
-      with w lct rct. _;
-      let v = Some?.v x;
-      rewrite each w as v;
-      rewrite each lct as (({ data = data; left = lct; right = rct }).left) in (is_tree lct ltree);
-      rewrite each rct as (({ data = data; left = lct; right = rct }).right) in (is_tree rct rtree);
-      fold (is_tree_cases (Some v) ft);
-      rewrite each (Some #(ref (node t)) v) as x;
+    T.Node data ltree rtree -> {
+      unfold (is_tree x (T.Node data ltree rtree));
+      with p _lct _rct. _;
+      fold (is_tree_cases (Some p) ft)
     }
   }
 }
@@ -176,13 +154,13 @@ fn is_tree_case_none (#t:Type) (x:tree_t t) (#l:T.tree t)
 requires is_tree x l ** pure (x == None)
 ensures  is_tree x l ** pure (l == T.Leaf)
 {
-  cases_of_is_tree x l;
-  rewrite each x as (None #(ref (node t)));
-  unfold (is_tree_cases None l);
-  intro_is_tree_nil x;
+  cases_of_is_tree None l;
+  unfold is_tree_cases;
+  intro_is_tree_leaf x;
 }
 
 ```
+
 ```pulse //is_list_case_some$
 ghost
 fn is_tree_case_some (#t:Type) (x:tree_t t) (v:node_ptr t) (#ft:T.tree t) 
@@ -195,9 +173,8 @@ ensures
     pure (ft == T.Node node.data ltree rtree)
   
 {
-  cases_of_is_tree x ft;
-  rewrite each x as (Some v);
-  unfold (is_tree_cases (Some v) ft);
+  cases_of_is_tree (Some v) ft;
+  unfold is_tree_cases;
 }
 ```
 ///////////////////////////////////////////////////////////////////////////////
@@ -215,641 +192,612 @@ ensures is_tree x 'l ** pure (n == T.height 'l)
     }
     Some vl -> {
       is_tree_case_some x vl;
-      with _node _ltree _rtree. _;
       let node = !vl;
-      rewrite each _node as node;
-      let left_tree_height = height node.left;
-      let right_tree_height = height node.right;
-      intro_is_tree_cons x vl;
-      if (left_tree_height > right_tree_height)
-      {
-        (left_tree_height + 1)
-      } 
-      else
-      {
-         (right_tree_height + 1)
+      let l_height = height node.left;
+      let r_height = height node.right;
+      intro_is_tree_node x vl;
+      if (l_height > r_height) {
+        (l_height + 1)
+      } else {
+        (r_height + 1)
       }
-       
     }
   }
 }
 ```
+
 ```pulse
-fn rec height_subtree (#t:Type0) (x:tree_t t) (k:nat)
+fn add_k_height (#t:Type0) (x:tree_t t) (k:nat)
 requires is_tree x 'l
 returns n:nat
 ensures is_tree x 'l ** pure (n == k + T.height 'l)
 {
+  let h = height x;
+  (h + k)
+}
+```
+
+```pulse
+fn is_empty (#t:Type) (x:tree_t t) 
+  requires is_tree x 'l
+  returns b:bool
+  ensures is_tree x 'l ** pure (b <==> ('l == T.Leaf))
+{
   match x {
     None -> {
       is_tree_case_none x;
-      k
+      true
     }
     Some vl -> {
       is_tree_case_some x vl;
-      with _node _ltree _rtree. _;
-      let n = !vl;
-      rewrite each _node as n;
-
-      let l1 = height n.left;
-      let l2 = height n.right;
-      let n1 = height_subtree n.left (1 + k);
-      let n2 = height_subtree n.right (1 + k);
-      intro_is_tree_cons x vl;
-      
-      (*if let l1 = height n.left;
-           let l2 = height n.right; is written after intro_is_tree_cons error is resulted. Why?*)
-      if (l1 > l2)
-      {
-         n1
-      }
-      else
-      {
-        n2
-      }
-      
+      intro_is_tree_node x vl;
+      false
     }
   }
 }
 ```
-```pulse
-fn is_empty (#t:Type) (x:tree_t t) 
-    requires is_tree x 'l
-    returns b:bool
-    ensures is_tree x 'l ** pure (b <==> ('l == T.Leaf))
-{
-    match x {
-        None -> {
-            is_tree_case_none x;
-            true
-        }
-        Some vl -> {
-            is_tree_case_some x vl;
-            intro_is_tree_cons x vl;
-            false
-        }
-    }
-}
-```
-let null_tree_t #t : tree_t t = None #(node_ptr t)
+let null_tree_t (t:Type0) : tree_t t = None
+
 
 ```pulse
-fn create (t:Type)
-    requires emp
-    returns x:tree_t t
-    ensures is_tree x T.Leaf
+fn create (t:Type0)
+  requires emp
+  returns x:tree_t t
+  ensures is_tree x T.Leaf
 {
-    intro_is_tree_nil #t null_tree_t;
-    null_tree_t #t
-}
-```
-```pulse
-fn node_cons (#t:Type) (v:t) (ltree:tree_t t) (rtree:tree_t t) 
-    requires is_tree ltree 'l  **
-             is_tree rtree 'r//functional equivalent of x is 'l; x is the tail of the constructed tree.
-    returns y:tree_t t
-    ensures is_tree y (T.Node v 'l 'r) ** ( pure (Some? y))
-{
-    let y = alloc { data=v; left =ltree; right = rtree };
-    rewrite each ltree as ({data = v; left = ltree; right = rtree}).left in (is_tree ltree 'l);
-    rewrite each rtree as ({data = v; left = ltree; right = rtree}).right in (is_tree rtree 'r);
-    intro_is_tree_cons (Some y) y;
-    Some y
+  let tree = null_tree_t t;
+  intro_is_tree_leaf tree;
+  tree
 }
 ```
 
-val get_left (#a: Type0) (n: node a) : tree_t a
-val get_right (#a: Type0) (n: node a) : tree_t a
-val get_data (#a: Type0) (n: node a) : a
+// ```pulse
+// fn node_cons (#t:Type0) (data:t) (ltree:tree_t t) (rtree:tree_t t) 
+//   requires is_tree ltree 'l  **
+//            is_tree rtree 'r  //functional equivalent of x is 'l; x is the tail of the constructed tree.
+//   returns y:tree_t t
+//   ensures is_tree y (T.Node v 'l 'r)
+// {
+//   let y = alloc { data=v; left =ltree; right = rtree };
+//   rewrite each ltree as ({data = v; left = ltree; right = rtree}).left in (is_tree ltree 'l);
+//   rewrite each rtree as ({data = v; left = ltree; right = rtree}).right in (is_tree rtree 'r);
+//   intro_is_tree_cons (Some y) y;
+//   Some y
+// }
+// ```
 
-let get_left #a n = n.left
-let get_right #a n = n.right
-let get_data #a n = n.data
+// val get_left (#a: Type0) (n: node a) : tree_t a
+// val get_right (#a: Type0) (n: node a) : tree_t a
+// val get_data (#a: Type0) (n: node a) : a
 
-
-val mk_node (#a: Type0) (data: a) (left right: tree_t a)
-    : Pure (node a)
-      (requires True)
-      (ensures (fun n -> get_left n == left /\ get_right n == right /\ get_data n == data))
-
-let mk_node #a data left right = {
-  data;
-  left;
-  right
-}
-
-
-
-/// Appends value [v] at the leftmost leaf of the tree that [ptr] points to.
-```pulse
-fn rec append_left_none (#t:Type0) (x:tree_t t) (v:t) 
-requires is_tree x 'l ** pure (None? x)
-returns y:tree_t t
-ensures is_tree x 'l  ** is_tree y (T.Node v T.Leaf T.Leaf)
-{
-  let left = create t;
-  let right = create t;
-  let y = node_cons v left right;
-      //intro_is_tree_nil x;
-      //fold (is_tree y (T.append_left 'l v));
-      //rewrite each (None #(ref (node t))) as x;
-      //y
-      //elim_is_tree_nil x;
-  //intro_is_tree_nil x;
-  //intro_is_tree_cons y;
-  y // How can we remove is_tree x 'l from the context?
-}
-```
+// let get_left #a n = n.left
+// let get_right #a n = n.right
+// let get_data #a n = n.data
 
 
-```pulse
-fn rec append_left (#t:Type0) (x:tree_t t) (v:t) 
-requires is_tree x 'l
-returns y:tree_t t
-ensures is_tree y  (T.append_left 'l v)
-{
-   match x {
-    None -> {
-      //current context: is_tree x (reveal 'l)
-      (*cond: requires is_tree x l ** pure (x == None)
-              ensures  is_tree x l ** pure (l == T.Leaf)*)
-      is_tree_case_none x;
-      //current context: is_tree x (reveal 'l) ** pure (reveal 'l == T.Leaf)
-      (*cond: requires is_tree x 'l ** pure ('l == T.Leaf)
-              ensures pure (x == None)*)
-      elim_is_tree_nil x;
-      //current cotext: pure (x == None)
+// val mk_node (#a: Type0) (data: a) (left right: tree_t a)
+//     : Pure (node a)
+//       (requires True)
+//       (ensures (fun n -> get_left n == left /\ get_right n == right /\ get_data n == data))
+
+// let mk_node #a data left right = {
+//   data;
+//   left;
+//   right
+// }
+
+
+
+// /// Appends value [v] at the leftmost leaf of the tree that [ptr] points to.
+// ```pulse
+// fn rec append_left_none (#t:Type0) (x:tree_t t) (v:t) 
+// requires is_tree x 'l ** pure (None? x)
+// returns y:tree_t t
+// ensures is_tree x 'l  ** is_tree y (T.Node v T.Leaf T.Leaf)
+// {
+//   let left = create t;
+//   let right = create t;
+//   let y = node_cons v left right;
+//       //intro_is_tree_nil x;
+//       //fold (is_tree y (T.append_left 'l v));
+//       //rewrite each (None #(ref (node t))) as x;
+//       //y
+//       //elim_is_tree_nil x;
+//   //intro_is_tree_nil x;
+//   //intro_is_tree_cons y;
+//   y // How can we remove is_tree x 'l from the context?
+// }
+// ```
+
+
+// ```pulse
+// fn rec append_left (#t:Type0) (x:tree_t t) (v:t) 
+// requires is_tree x 'l
+// returns y:tree_t t
+// ensures is_tree y  (T.append_left 'l v)
+// {
+//    match x {
+//     None -> {
+//       //current context: is_tree x (reveal 'l)
+//       (*cond: requires is_tree x l ** pure (x == None)
+//               ensures  is_tree x l ** pure (l == T.Leaf)*)
+//       is_tree_case_none x;
+//       //current context: is_tree x (reveal 'l) ** pure (reveal 'l == T.Leaf)
+//       (*cond: requires is_tree x 'l ** pure ('l == T.Leaf)
+//               ensures pure (x == None)*)
+//       elim_is_tree_nil x;
+//       //current cotext: pure (x == None)
       
-      let left = create t;
-      let right = create t;
-      //Current context: is_tree right T.Leaf ** is_tree left T.Leaf
+//       let left = create t;
+//       let right = create t;
+//       //Current context: is_tree right T.Leaf ** is_tree left T.Leaf
     
-      let y = node_cons v left right;
-      //Current context:
-      //is_tree y (T.Node v (reveal (hide T.Leaf)) (reveal (hide T.Leaf))) **
-      //pure (Some? y)
+//       let y = node_cons v left right;
+//       //Current context:
+//       //is_tree y (T.Node v (reveal (hide T.Leaf)) (reveal (hide T.Leaf))) **
+//       //pure (Some? y)
     
-      let np = Some?.v y;
+//       let np = Some?.v y;
       
-    //Current context:
-    //pure (np == y.v) **
-    //is_tree y (T.Node v (reveal (hide T.Leaf)) (reveal (hide T.Leaf)))
-     (*cond: requires is_tree x ft ** pure (x == Some v)
-             ensures  
-                exists* (node:node t) (ltree:T.tree t) (rtree:T.tree t).
-                pts_to v node **
-                is_tree node.left ltree **
-                is_tree node.right rtree **
-                pure (ft == T.Node node.data ltree rtree)*)
-     is_tree_case_some y np;
+//     //Current context:
+//     //pure (np == y.v) **
+//     //is_tree y (T.Node v (reveal (hide T.Leaf)) (reveal (hide T.Leaf)))
+//      (*cond: requires is_tree x ft ** pure (x == Some v)
+//              ensures  
+//                 exists* (node:node t) (ltree:T.tree t) (rtree:T.tree t).
+//                 pts_to v node **
+//                 is_tree node.left ltree **
+//                 is_tree node.right rtree **
+//                 pure (ft == T.Node node.data ltree rtree)*)
+//      is_tree_case_some y np;
 
-     (*Current context:
-               (exists* (node:node t) (ltree:T.tree t) (rtree:T.tree t).
-               pts_to np node ** 
-               is_tree node.left ltree ** 
-               is_tree node.right rtree **
-               pure (T.Node v (reveal (hide T.Leaf)) (reveal (hide T.Leaf)) ==
-               T.Node node.data ltree rtree))*)
+//      (*Current context:
+//                (exists* (node:node t) (ltree:T.tree t) (rtree:T.tree t).
+//                pts_to np node ** 
+//                is_tree node.left ltree ** 
+//                is_tree node.right rtree **
+//                pure (T.Node v (reveal (hide T.Leaf)) (reveal (hide T.Leaf)) ==
+//                T.Node node.data ltree rtree))*)
     
-      intro_is_tree_cons y np;
+//       intro_is_tree_cons y np;
 
-      (*Current context:
-        is_tree y (T.Node (reveal node).data (reveal ltree) (reveal rtree)*)
-      (*requires
-        pts_to v node **
-        is_tree node.left ltree **
-        is_tree node.right rtree **
-        pure (ct == Some v)
-      ensures
-        is_tree ct (T.Node node.data ltree rtree)*)
-      y 
-    }
-    Some vl -> {
-      //current context: is_tree x (reveal 'l)
-      let np = Some?.v x;
-      (*Current context:
-        pure (np == x.v) ** is_tree x (reveal 'l)*)
-      is_tree_case_some x np;
-      (*Current context:
-        (exists* (node:node t) (ltree:T.tree t) (rtree:T.tree t).
-         pts_to np node ** is_tree node.left ltree ** is_tree node.right rtree **
-         pure (reveal 'l == T.Node node.data ltree rtree))*)
-      with _node _ltree _rtree._;
-      (*Current context:
-        pts_to np (reveal node) **
-        is_tree (reveal node).left (reveal ltree) **
-        is_tree (reveal node).right (reveal rtree) **
-        pure (reveal 'l == T.Node (reveal node).data (reveal ltree) (reveal rtree))*)
-      let node = !np;
-      (*Current context:
-         pts_to np (reveal node) **
-         pure (reveal node == node) **
-        is_tree (reveal node).left (reveal ltree) **
-        is_tree (reveal node).right (reveal rtree)*)
+//       (*Current context:
+//         is_tree y (T.Node (reveal node).data (reveal ltree) (reveal rtree)*)
+//       (*requires
+//         pts_to v node **
+//         is_tree node.left ltree **
+//         is_tree node.right rtree **
+//         pure (ct == Some v)
+//       ensures
+//         is_tree ct (T.Node node.data ltree rtree)*)
+//       y 
+//     }
+//     Some vl -> {
+//       //current context: is_tree x (reveal 'l)
+//       let np = Some?.v x;
+//       (*Current context:
+//         pure (np == x.v) ** is_tree x (reveal 'l)*)
+//       is_tree_case_some x np;
+//       (*Current context:
+//         (exists* (node:node t) (ltree:T.tree t) (rtree:T.tree t).
+//          pts_to np node ** is_tree node.left ltree ** is_tree node.right rtree **
+//          pure (reveal 'l == T.Node node.data ltree rtree))*)
+//       with _node _ltree _rtree._;
+//       (*Current context:
+//         pts_to np (reveal node) **
+//         is_tree (reveal node).left (reveal ltree) **
+//         is_tree (reveal node).right (reveal rtree) **
+//         pure (reveal 'l == T.Node (reveal node).data (reveal ltree) (reveal rtree))*)
+//       let node = !np;
+//       (*Current context:
+//          pts_to np (reveal node) **
+//          pure (reveal node == node) **
+//         is_tree (reveal node).left (reveal ltree) **
+//         is_tree (reveal node).right (reveal rtree)*)
       
-      rewrite each _node as node;
+//       rewrite each _node as node;
 
-      (*Current context:
-        is_tree node.right (reveal rtree) **
-        is_tree node.left (reveal ltree) ** pts_to np node*)
+//       (*Current context:
+//         is_tree node.right (reveal rtree) **
+//         is_tree node.left (reveal ltree) ** pts_to np node*)
 
       
-      let left_new = append_left node.left v;
+//       let left_new = append_left node.left v;
       
-      (*Current context:
-        is_tree left_new (T.append_left (reveal ltree) v) **
-        pts_to np node ** is_tree node.right (reveal rtree)*)
-      np := {node with left = left_new};
+//       (*Current context:
+//         is_tree left_new (T.append_left (reveal ltree) v) **
+//         pts_to np node ** is_tree node.right (reveal rtree)*)
+//       np := {node with left = left_new};
       
        
-      (*Current context:
-        pts_to np (Mknode node.data left_new node.right) **
-        is_tree node.right (reveal rtree) **
-        is_tree left_new (T.append_left (reveal ltree) v)*)
+//       (*Current context:
+//         pts_to np (Mknode node.data left_new node.right) **
+//         is_tree node.right (reveal rtree) **
+//         is_tree left_new (T.append_left (reveal ltree) v)*)
       
-       rewrite each left_new as ({ node with left = left_new }).left in (is_tree left_new ((T.append_left (reveal _ltree) v)));
+//        rewrite each left_new as ({ node with left = left_new }).left in (is_tree left_new ((T.append_left (reveal _ltree) v)));
       
 
-      (*Current context:
-         is_tree (Mknode node.data left_new node.right).left
-                (T.append_left (reveal ltree) v) **
-         pts_to np (Mknode node.data left_new node.right) **
-         is_tree node.right (reveal rtree)*)
+//       (*Current context:
+//          is_tree (Mknode node.data left_new node.right).left
+//                 (T.append_left (reveal ltree) v) **
+//          pts_to np (Mknode node.data left_new node.right) **
+//          is_tree node.right (reveal rtree)*)
 
-       rewrite each node.right as ({ node with left = left_new }).right in (is_tree node.right _rtree);
+//        rewrite each node.right as ({ node with left = left_new }).right in (is_tree node.right _rtree);
        
-      (*Current context:
-         is_tree (Mknode node.data left_new node.right).right (reveal rtree) **
-         is_tree (Mknode node.data left_new node.right).left
-                  (T.append_left (reveal ltree) v) **
-        pts_to np (Mknode node.data left_new node.right)*)
+//       (*Current context:
+//          is_tree (Mknode node.data left_new node.right).right (reveal rtree) **
+//          is_tree (Mknode node.data left_new node.right).left
+//                   (T.append_left (reveal ltree) v) **
+//         pts_to np (Mknode node.data left_new node.right)*)
        
-       intro_is_tree_cons x np;
+//        intro_is_tree_cons x np;
 
-       (*Current context:
-        is_tree x
-             (T.Node (Mknode node.data left_new node.right).data
-                  (T.append_left (reveal ltree) v)
-                  (reveal rtree))*)
-       //show_proof_state;
+//        (*Current context:
+//         is_tree x
+//              (T.Node (Mknode node.data left_new node.right).data
+//                   (T.append_left (reveal ltree) v)
+//                   (reveal rtree))*)
+//        //show_proof_state;
 
-      x
-    }
-  }
-} 
-```
+//       x
+//     }
+//   }
+// } 
+// ```
 
 
-```pulse
-fn rec append_right (#t:Type0) (x:tree_t t) (v:t) 
-requires is_tree x 'l
-returns y:tree_t t
-ensures is_tree y  (T.append_right 'l v)
-{
-   match x {
-    None -> {
+// ```pulse
+// fn rec append_right (#t:Type0) (x:tree_t t) (v:t) 
+// requires is_tree x 'l
+// returns y:tree_t t
+// ensures is_tree y  (T.append_right 'l v)
+// {
+//    match x {
+//     None -> {
       
-      is_tree_case_none x;
+//       is_tree_case_none x;
       
-      elim_is_tree_nil x;
+//       elim_is_tree_nil x;
      
-      let left = create t;
-      let right = create t;
+//       let left = create t;
+//       let right = create t;
       
     
-      let y = node_cons v left right;
+//       let y = node_cons v left right;
       
-      let np = Some?.v y;
+//       let np = Some?.v y;
       
-      is_tree_case_some y np;
+//       is_tree_case_some y np;
 
-      intro_is_tree_cons y np;
+//       intro_is_tree_cons y np;
       
-      y 
-    }
-    Some vl -> {
+//       y 
+//     }
+//     Some vl -> {
       
-      let np = Some?.v x;
+//       let np = Some?.v x;
       
-      is_tree_case_some x np;
+//       is_tree_case_some x np;
       
-      with _node _ltree _rtree._;
+//       with _node _ltree _rtree._;
       
-      let node = !np;
+//       let node = !np;
       
-      rewrite each _node as node;
+//       rewrite each _node as node;
 
-      let right_new = append_right node.right v;
+//       let right_new = append_right node.right v;
       
-      np := {node with right = right_new};
+//       np := {node with right = right_new};
       
-      rewrite each right_new as ({ node with right = right_new }).right in (is_tree right_new ((T.append_right (reveal _rtree) v)));
+//       rewrite each right_new as ({ node with right = right_new }).right in (is_tree right_new ((T.append_right (reveal _rtree) v)));
       
-      rewrite each node.left as ({node with right = right_new}).left in (is_tree node.left _ltree);
+//       rewrite each node.left as ({node with right = right_new}).left in (is_tree node.left _ltree);
       
-      intro_is_tree_cons x np;
+//       intro_is_tree_cons x np;
       
-      x
-    }
-  }
-} 
-```
+//       x
+//     }
+//   }
+// } 
+// ```
 
-```pulse
-fn node_data (#t:Type) (x:tree_t t) 
-    requires is_tree x 'l  ** (pure (Some? x))
-    returns v:t
-    ensures is_tree x 'l 
-{
-  let np = Some?.v x;
+// ```pulse
+// fn node_data (#t:Type) (x:tree_t t) 
+//     requires is_tree x 'l  ** (pure (Some? x))
+//     returns v:t
+//     ensures is_tree x 'l 
+// {
+//   let np = Some?.v x;
       
-  is_tree_case_some x np;
+//   is_tree_case_some x np;
       
-  with _node _ltree _rtree._;
+//   with _node _ltree _rtree._;
       
-  let node = !np;
+//   let node = !np;
       
-  rewrite each _node as node;
+//   rewrite each _node as node;
 
-  let v = node.data;
+//   let v = node.data;
   
-  intro_is_tree_cons x np;
-  v
-}
-```
+//   intro_is_tree_cons x np;
+//   v
+// }
+// ```
 
-```pulse
-fn rec is_mem (#t:eqtype) (x:tree_t t) (v: t)
-    requires is_tree x 'l
-    returns b:bool
-    ensures is_tree x 'l ** pure (b <==> (T.mem 'l v))
-{
-   match x {
-        None -> {
-            is_tree_case_none x;
-            false
-        }
-        Some vl -> {
-            //let dat = node_data x;
-            is_tree_case_some x vl;
-            with _node _ltree _rtree. _;
-            let n = !vl;
-            rewrite each _node as n;
+// ```pulse
+// fn rec is_mem (#t:eqtype) (x:tree_t t) (v: t)
+//     requires is_tree x 'l
+//     returns b:bool
+//     ensures is_tree x 'l ** pure (b <==> (T.mem 'l v))
+// {
+//    match x {
+//         None -> {
+//             is_tree_case_none x;
+//             false
+//         }
+//         Some vl -> {
+//             //let dat = node_data x;
+//             is_tree_case_some x vl;
+//             with _node _ltree _rtree. _;
+//             let n = !vl;
+//             rewrite each _node as n;
 
-            let dat = n.data;
+//             let dat = n.data;
             
-            if (dat = v) 
-            {
-              intro_is_tree_cons x vl;
-              true
-            }
-            else{
-              let b1 = is_mem n.left v;
-              let b2 = is_mem n.right v;
+//             if (dat = v) 
+//             {
+//               intro_is_tree_cons x vl;
+//               true
+//             }
+//             else{
+//               let b1 = is_mem n.left v;
+//               let b2 = is_mem n.right v;
 
-              let b3 = b1 || b2;
-              intro_is_tree_cons x vl;
-              b3;
+//               let b3 = b1 || b2;
+//               intro_is_tree_cons x vl;
+//               b3;
               
-            }
-        }
-    }
-}
-```
-```pulse //cases_of_is_tree$
-ghost
-fn cases_of_is_tree_reverse #t (x:tree_t t) (ft:T.tree t)
-requires  is_tree_cases x ft
+//             }
+//         }
+//     }
+// }
+// ```
+// ```pulse //cases_of_is_tree$
+// ghost
+// fn cases_of_is_tree_reverse #t (x:tree_t t) (ft:T.tree t)
+// requires  is_tree_cases x ft
 
-ensures is_tree x ft
-{
-  admit()
-}
-```
+// ensures is_tree x ft
+// {
+//   admit()
+// }
+// ```
 
-```pulse //is_list_case_some$
-ghost
-fn is_tree_case_some1 (#t:Type) (x:tree_t t) (v:node_ptr t) (#ft:T.tree t) 
-requires 
-exists* (node:node t) (ltree:T.tree t) (rtree:T.tree t).
-    is_tree x ft **
-    pts_to v node **
-    is_tree node.left ltree **
-    is_tree node.right rtree **
-    pure (ft == T.Node node.data ltree rtree)
+// ```pulse //is_list_case_some$
+// ghost
+// fn is_tree_case_some1 (#t:Type) (x:tree_t t) (v:node_ptr t) (#ft:T.tree t) 
+// requires 
+// exists* (node:node t) (ltree:T.tree t) (rtree:T.tree t).
+//     is_tree x ft **
+//     pts_to v node **
+//     is_tree node.left ltree **
+//     is_tree node.right rtree **
+//     pure (ft == T.Node node.data ltree rtree)
 
-ensures  is_tree x ft ** pure (x == Some v)
+// ensures  is_tree x ft ** pure (x == Some v)
    
   
-{
+// {
   
-  fold(is_tree_cases (Some v) ft);
-  //rewrite each (Some v) as x;
-  //show_proof_state;
-  cases_of_is_tree_reverse (Some v) ft;
-  //show_proof_state;
-  assert (is_tree x ft);
+//   fold(is_tree_cases (Some v) ft);
+//   //rewrite each (Some v) as x;
+//   //show_proof_state;
+//   cases_of_is_tree_reverse (Some v) ft;
+//   //show_proof_state;
+//   assert (is_tree x ft);
   
-  //show_proof_state;
+//   //show_proof_state;
   
-  admit()
-}
-```
+//   admit()
+// }
+// ```
 
 
-(*cases_of_is_tree x ft;
-  rewrite each x as (Some v);
-  unfold (is_tree_cases (Some v) ft);*)
+// (*cases_of_is_tree x ft;
+//   rewrite each x as (Some v);
+//   unfold (is_tree_cases (Some v) ft);*)
+
+// ```pulse
+// ghost
+// fn non_empty_tree (#t:Type0) (x:tree_t t) (ft:T.tree t)
+// requires is_tree x ft ** pure (T.Node? ft)
+// ensures is_tree x ft ** pure (Some? x)
+// {
+//     match x {
+//       None -> {
+//         intro_is_tree_nil x;
+//         show_proof_state;
+//         admit()
+//       }
+//       Some vl -> {
+//         admit()
+//       }
+//     }
+   
+//     (*n intro_is_tree_cons (#t:Type0) (ct:tree_t t) (v:node_ptr t) (#node:node t) (#ltree:T.tree t) (#rtree:T.tree t)
+//   requires
+//   pts_to v node **
+//   is_tree node.left ltree **
+//   is_tree node.right rtree **
+//   pure (ct == Some v)*)
+
+//     (*elim_is_tree_cons x _ (T.Node?.data 'l) (T.Node?.left 'l) (T.Node?.right 'l);
+
+//     with v lct rct. _;
+//     with n left right. assert (pts_to v n ** is_tree lct left ** is_tree rct right);
+    
+//     (*Current context:
+//     pts_to (reveal p) (Mknode (reveal 'l).data (reveal lct) (reveal rct)) **
+//     is_tree (reveal lct) (reveal 'l).left **
+//     is_tree (reveal rct) (reveal 'l).right*)
+
+    
+//     rewrite each (reveal lct) as n.left;
+//     show_proof_state;
+//     // show_proof_state;
+
+//     (*Current context:
+//     is_tree (Mknode (reveal 'l).data (reveal lct) (reveal rct)).left
+//       (reveal 'l).left **
+//     pts_to (reveal p)
+//       (Mknode (reveal 'l).data
+//           (Mknode (reveal 'l).data (reveal lct) (reveal rct)).left
+//           (reveal rct)) **
+//     is_tree (reveal rct) (reveal 'l).right*)
+    
+//     rewrite each rct as n.right;
+//     show_proof_state;
+    
+//     (*Current context:
+//     is_tree (Mknode (reveal 'l).data (reveal lct) (reveal rct)).right
+//       (reveal 'l).right **
+
+//     pts_to (reveal p)
+//       (Mknode (reveal 'l).data
+//           (Mknode (reveal 'l).data
+//               (reveal lct)
+//               (Mknode (reveal 'l).data (reveal lct) (reveal rct)).right)
+//             .left
+//           (Mknode (reveal 'l).data (reveal lct) (reveal rct)).right) **
+
+//     is_tree (Mknode (reveal 'l).data
+//           (reveal lct)
+//           (Mknode (reveal 'l).data (reveal lct) (reveal rct)).right)
+//         .left
+//       (reveal 'l).left
+
+
+//     show_proof_state;
+    
+    
+    
+
+   
+//     //show_proof_state;
+//     //intro_is_tree_cons x v #n #left #right;*)*)
+// }
+
+// ```
+
+// (*```pulse //non_empty_list$
+// ghost
+// fn non_empty_list (#t:Type0) (x:llist t)
+// requires is_list x 'l ** pure (Cons? 'l)
+// ensures is_list x 'l ** pure (Some? x)
+// {
+//     elim_is_list_cons x _ (Cons?.hd 'l) (Cons?.tl 'l);
+//     with v tail. _;
+//     with n tl. assert (pts_to v n ** is_list tail tl);
+//     rewrite each tail as n.tail;
+//     intro_is_list_cons x v #n #tl;
+// }
+// ```*)
+
+// (*n intro_is_tree_cons (#t:Type0) (ct:tree_t t) (v:node_ptr t) (#node:node t) (#ltree:T.tree t) (#rtree:T.tree t)
+// requires
+//   pts_to v node **
+//   is_tree node.left ltree **
+//   is_tree node.right rtree **
+//   pure (ct == Some v)*)
+
+// (*fn elim_is_tree_cons (#t:Type0) (ct:tree_t t) (ft:T.tree t) (data:t) (ltree:T.tree t) (rtree:T.tree t)
+// requires is_tree ct ft ** pure (ft == T.Node data ltree rtree)*)
+
+
 
 ```pulse
-ghost
-fn non_empty_tree (#t:Type0) (x:tree_t t) (ft:T.tree t)
-requires is_tree x ft ** pure (T.Node? ft)
-ensures is_tree x ft ** pure (Some? x)
-{
-    match x {
-      None -> {
-        intro_is_tree_nil x;
-        show_proof_state;
-        admit()
-      }
-      Some vl -> {
-        admit()
-      }
-    }
-   
-    (*n intro_is_tree_cons (#t:Type0) (ct:tree_t t) (v:node_ptr t) (#node:node t) (#ltree:T.tree t) (#rtree:T.tree t)
-  requires
-  pts_to v node **
-  is_tree node.left ltree **
-  is_tree node.right rtree **
-  pure (ct == Some v)*)
-
-    (*elim_is_tree_cons x _ (T.Node?.data 'l) (T.Node?.left 'l) (T.Node?.right 'l);
-
-    with v lct rct. _;
-    with n left right. assert (pts_to v n ** is_tree lct left ** is_tree rct right);
-    
-    (*Current context:
-    pts_to (reveal p) (Mknode (reveal 'l).data (reveal lct) (reveal rct)) **
-    is_tree (reveal lct) (reveal 'l).left **
-    is_tree (reveal rct) (reveal 'l).right*)
-
-    
-    rewrite each (reveal lct) as n.left;
-    show_proof_state;
-    // show_proof_state;
-
-    (*Current context:
-    is_tree (Mknode (reveal 'l).data (reveal lct) (reveal rct)).left
-      (reveal 'l).left **
-    pts_to (reveal p)
-      (Mknode (reveal 'l).data
-          (Mknode (reveal 'l).data (reveal lct) (reveal rct)).left
-          (reveal rct)) **
-    is_tree (reveal rct) (reveal 'l).right*)
-    
-    rewrite each rct as n.right;
-    show_proof_state;
-    
-    (*Current context:
-    is_tree (Mknode (reveal 'l).data (reveal lct) (reveal rct)).right
-      (reveal 'l).right **
-
-    pts_to (reveal p)
-      (Mknode (reveal 'l).data
-          (Mknode (reveal 'l).data
-              (reveal lct)
-              (Mknode (reveal 'l).data (reveal lct) (reveal rct)).right)
-            .left
-          (Mknode (reveal 'l).data (reveal lct) (reveal rct)).right) **
-
-    is_tree (Mknode (reveal 'l).data
-          (reveal lct)
-          (Mknode (reveal 'l).data (reveal lct) (reveal rct)).right)
-        .left
-      (reveal 'l).left
-
-
-    show_proof_state;
-    
-    
-    
-
-   
-    //show_proof_state;
-    //intro_is_tree_cons x v #n #left #right;*)*)
-}
-
-```
-
-(*```pulse //non_empty_list$
-ghost
-fn non_empty_list (#t:Type0) (x:llist t)
-requires is_list x 'l ** pure (Cons? 'l)
-ensures is_list x 'l ** pure (Some? x)
-{
-    elim_is_list_cons x _ (Cons?.hd 'l) (Cons?.tl 'l);
-    with v tail. _;
-    with n tl. assert (pts_to v n ** is_list tail tl);
-    rewrite each tail as n.tail;
-    intro_is_list_cons x v #n #tl;
-}
-```*)
-
-(*n intro_is_tree_cons (#t:Type0) (ct:tree_t t) (v:node_ptr t) (#node:node t) (#ltree:T.tree t) (#rtree:T.tree t)
-requires
-  pts_to v node **
-  is_tree node.left ltree **
-  is_tree node.right rtree **
-  pure (ct == Some v)*)
-
-(*fn elim_is_tree_cons (#t:Type0) (ct:tree_t t) (ft:T.tree t) (data:t) (ltree:T.tree t) (rtree:T.tree t)
-requires is_tree ct ft ** pure (ft == T.Node data ltree rtree)*)
-
-
-
-```pulse
-fn rec rotate_left (#t:Type0) (x:tree_t t)
-requires is_tree x 'l ** (pure (Some? (T.rotate_left 'l)))
-        (pure (Some? x)) **
-        (pure (Some? rtr)) ** pure (rtree == T.Node data_r ltree_r rtree_r) 
+fn rec rotate_left (#t:Type0) (x:tree_t t) (#l:T.tree t{ Some? (T.rotate_left l) })
+requires is_tree x l
 returns y:tree_t t 
-ensures exists* (ft:T.tree t).
-  pure (Some ft == T.rotate_left 'l) ** (is_tree y ft)
+ensures (is_tree y (Some?.v (T.rotate_left l)))
 {
   
-  //get the node, node_x from the tree x --- T.Node data_x left_x right_x
 
-   let np = Some?.v x;
+
+  admit ()
+  // //get the node, node_x from the tree x --- T.Node data_x left_x right_x
+
+  //  let np = Some?.v x;
    
-   is_tree_case_some x np;
+  //  is_tree_case_some x np;
       
-   with _node _ltree _rtree._;
+  //  with _node _ltree _rtree._;
       
-   let node_x = !np;
+  //  let node_x = !np;
       
-   rewrite each _node as node_x;
+  //  rewrite each _node as node_x;
 
-   (*Current context:
-    is_tree node.right (reveal rtree) **
-    is_tree node.left (reveal ltree) ** pts_to np node ** is_tree rtr rtree*)
+  //  (*Current context:
+  //   is_tree node.right (reveal rtree) **
+  //   is_tree node.left (reveal ltree) ** pts_to np node ** is_tree rtr rtree*)
 
-   //get the data, data_x from the node_x --- data_x
-   let data_x = node_x.data;
+  //  //get the data, data_x from the node_x --- data_x
+  //  let data_x = node_x.data;
    
-   (* Current context:
-    pure (data_x == node_x.data) **
-    is_tree node_x.right (reveal rtree) **
-    is_tree node_x.left (reveal ltree) ** pts_to np node_x ** is_tree rtr rtree*)
+  //  (* Current context:
+  //   pure (data_x == node_x.data) **
+  //   is_tree node_x.right (reveal rtree) **
+  //   is_tree node_x.left (reveal ltree) ** pts_to np node_x ** is_tree rtr rtree*)
 
    
 
-  //get the node, node_r from the right tree of x, node_x.right --- T.Node data_xr left_xr right_xr
-  let r_np = Some?.v rtr;
-  (*Current context:
-    pure (r_np == rtr.v) **
-    is_tree node_x.right (reveal rtree) **
-    is_tree node_x.left (reveal ltree) ** pts_to np node_x ** is_tree rtr rtree*)
+  // //get the node, node_r from the right tree of x, node_x.right --- T.Node data_xr left_xr right_xr
+  // let r_np = Some?.v rtr;
+  // (*Current context:
+  //   pure (r_np == rtr.v) **
+  //   is_tree node_x.right (reveal rtree) **
+  //   is_tree node_x.left (reveal ltree) ** pts_to np node_x ** is_tree rtr rtree*)
   
-  is_tree_case_some rtr r_np;
-  (*Current context:
-    (exists* (node:node t) (ltree:T.tree t) (rtree:T.tree t).
-      pts_to r_np node ** is_tree node.left ltree ** is_tree node.right rtree **
-      pure (rtree == T.Node node.data ltree rtree)) **
-    is_tree node_x.right (reveal rtree) **
-    is_tree node_x.left (reveal ltree) ** pts_to np node_x*)
+  // is_tree_case_some rtr r_np;
+  // (*Current context:
+  //   (exists* (node:node t) (ltree:T.tree t) (rtree:T.tree t).
+  //     pts_to r_np node ** is_tree node.left ltree ** is_tree node.right rtree **
+  //     pure (rtree == T.Node node.data ltree rtree)) **
+  //   is_tree node_x.right (reveal rtree) **
+  //   is_tree node_x.left (reveal ltree) ** pts_to np node_x*)
   
-  show_proof_state;
+  // show_proof_state;
       
-   with _node_r _ltree_r _rtree_r._;
+  //  with _node_r _ltree_r _rtree_r._;
       
-   let node_r = !r_np;
+  //  let node_r = !r_np;
       
-   rewrite each _node_r as node_r;
+  //  rewrite each _node_r as node_r;
   
   
-  show_proof_state;
-  //get the data, data_r from node_r --- data_xr
+  // show_proof_state;
+  // //get the data, data_r from node_r --- data_xr
 
-  //create subnode with data_x, 
-  // left tree as node.left
-  // right tree as (node_r).left 
+  // //create subnode with data_x, 
+  // // left tree as node.left
+  // // right tree as (node_r).left 
 
-  // create a new node with data as data_r, left as x
-  // right node_r.right;
+  // // create a new node with data as data_r, left as x
+  // // right node_r.right;
 
-  //write in (node_x).right new node
+  // //write in (node_x).right new node
 
-  //write in x subnode
+  // //write in x subnode
 
-  //pack_tree x (node_x.left) (node_r.left);
+  // //pack_tree x (node_x.left) (node_r.left);
 
-  //pack_tree (node_x.right) x (node_r.right);
+  // //pack_tree (node_x.right) x (node_r.right);
 
-  // (node_x.right)
+  // // (node_x.right)
 
-  admit()
+  // admit()
  
 }
 ```
